Cedille/Lemma/Confluence.lean
@@ -1,8 +1,440 @@
 
 import Cedille.Def
+import Cedille.Lemma.Basic
+import Cedille.Lemma.Refold
+import Cedille.Lemma.Erasure
+import Cedille.Lemma.Inversion
+import Cedille.Lemma.Syntax
+import Cedille.Lemma.Substitution
+import Cedille.Lemma.Red
+
+-- based heavily off https://plfa.inf.ed.ac.uk/Confluence/
 
 namespace Cedille
 
-  theorem confluence : t -β>* t1 -> t -β>* t2 -> ∃ z, t1 -β>* z ∧ t2 -β>* z := sorry
+  def parp (t : Term n) : Term n :=
+    match t with
+    | Syntax.const k => const k
+    | Syntax.bound i => bound i
+    | Syntax.free x => free x
+    | Syntax.ctor (Constructor.app _)
+      (Syntax.bind (Binder.lam _) _t1 t2)
+      t3
+      (Syntax.const Constant.kindU)
+      => [_:= parp t3](parp t2)
+    | Syntax.ctor Constructor.fst
+      (Syntax.ctor Constructor.pair u1 _u2 _u3)
+      (Syntax.const Constant.kindU)
+      (Syntax.const Constant.kindU)
+      => parp u1
+    | Syntax.ctor Constructor.fst
+      (Syntax.ctor Constructor.phi u1 _u2 _u3)
+      (Syntax.const Constant.kindU)
+      (Syntax.const Constant.kindU)
+      => parp u1
+    | Syntax.ctor Constructor.snd
+      (Syntax.ctor Constructor.pair _u1 u2 _u3)
+      (Syntax.const Constant.kindU)
+      (Syntax.const Constant.kindU)
+      => parp u2
+    | Syntax.ctor Constructor.eqind
+      _t1
+      _t2
+      (Syntax.ctor Constructor.jω
+        (Syntax.ctor Constructor.refl
+          v1
+          (Syntax.const Constant.kindU)
+          (Syntax.const Constant.kindU))
+        u2
+        (Syntax.const Constant.kindU))
+      => app m0 (parp u2) (parp v1)
+    | Syntax.ctor Constructor.promote
+      (Syntax.ctor Constructor.refl
+        (Syntax.ctor Constructor.fst
+          v1
+          (Syntax.const Constant.kindU)
+          (Syntax.const Constant.kindU))
+        (Syntax.const Constant.kindU)
+        (Syntax.const Constant.kindU))
+      (Syntax.const Constant.kindU)
+      (Syntax.const Constant.kindU)
+      => refl (parp v1)
+    | Syntax.bind k t1 t2 => Syntax.bind k (parp t1) (parp t2)
+    | Syntax.ctor k t1 t2 t3 => Syntax.ctor k (parp t1) (parp t2) (parp t3)
+
+  inductive ParRed {n : Nat} : Term n -> Term n -> Prop where
+  | beta {S : FvSet!} :
+    ParRed t1 t1' ->
+    (∀ x, x ∉ S -> ParRed ({_|-> x}t2) ({_|-> x}t2')) ->
+    ParRed t3 t3' ->
+    ParRed (app m (lam m t1 t2) t3) ([_:= t3']t2')
+  | fst :
+    ParRed t1 t1' ->
+    ParRed t2 t2' ->
+    ParRed t3 t3' ->
+    ParRed (fst (pair t1 t2 t3)) t1'
+  | snd :
+    ParRed t1 t1' ->
+    ParRed t2 t2' ->
+    ParRed t3 t3' ->
+    ParRed (snd (pair t1 t2 t3)) t2'
+  | eqind :
+    ParRed t1 t1' ->
+    ParRed t2 t2' ->
+    ParRed t3 t3' ->
+    ParRed t4 t4' ->
+    ParRed t5 t5' ->
+    ParRed t6 t6' ->
+    ParRed (J t1 t2 t3 t4 (refl t5) t6) (t6' @0 t5')
+  | promote :
+    ParRed t t' ->
+    ParRed (promote (refl (fst t))) (refl t')
+  | phi :
+    ParRed t1 t1' ->
+    ParRed t2 t2' ->
+    ParRed t3 t3' ->
+    ParRed (fst (phi t1 t2 t3)) t1'
+  | bind {S : FvSet!} :
+    ParRed t1 t1' ->
+    ((x : Name) -> x ∉ S -> ParRed ({_|-> x}t2) ({_|-> x}t2')) ->
+    ParRed (Syntax.bind k t1 t2) (Syntax.bind k t1' t2')
+  | ctor :
+    ParRed t1 t1' ->
+    ParRed t2 t2' ->
+    ParRed t3 t3' ->
+    ParRed (Syntax.ctor k t1 t2 t3) (Syntax.ctor k t1' t2' t3')
+  | const : ParRed (const K) (const K)
+  | free : ParRed (free x) (free x)
+  | bound : ParRed (bound i) (bound i)
+
+  notation:150 t1:150 " -p> " t2:150 => @ParRed 0 t1 t2
+
+  inductive ParRedStar : Term 0 -> Term 0 -> Prop where
+  | refl : ParRedStar t t
+  | step : t1 -p> t2 -> ParRedStar t2 t3 -> ParRedStar t1 t3
+
+  notation:150 t1:150 " -p>* " t2:150 => ParRedStar t1 t2
+
+  namespace ParRed
+
+    lemma refl_bind_open (x : Name) : x ∉ fv t -> ParRed t t -> ParRed ({_|-> x}t) ({_|-> x}t) := by {
+      sorry
+    }
+
+    lemma refl_n : ParRed t t := by {
+      induction t
+      case bound => apply ParRed.bound
+      case free => apply ParRed.free
+      case const => apply ParRed.const
+      case bind n1 n2 b t1 t2 ih1 ih2 => {
+        apply ParRed.bind; apply ih1
+        swap; exact (fv t2)
+        intro x xn
+        apply refl_bind_open x xn ih2
+      }
+      case ctor n1 n2 k t1 t2 t3 ih1 ih2 ih3 => {
+        apply ParRed.ctor; apply ih1; apply ih2; apply ih3
+      }
+    }
+
+    lemma refl : t -p> t := refl_n
+
+  end ParRed
+
+  lemma red_implies_par_step : t -β> s -> t -p> s := by {
+    intro step
+    induction step
+    case beta m t1 t2 t3 => {
+      apply ParRed.beta; apply ParRed.refl
+      intro x _; apply ParRed.refl
+      apply ParRed.refl; exact []
+    }
+    case fst => {
+      apply ParRed.fst
+      apply ParRed.refl; apply ParRed.refl; apply ParRed.refl
+    }
+    case snd => {
+      apply ParRed.snd
+      apply ParRed.refl; apply ParRed.refl; apply ParRed.refl
+    }
+    case eqind => {
+      apply ParRed.eqind
+      apply ParRed.refl; apply ParRed.refl; apply ParRed.refl
+      apply ParRed.refl; apply ParRed.refl; apply ParRed.refl
+    }
+    case promote => {
+      apply ParRed.promote; apply ParRed.refl
+    }
+    case phi => {
+      apply ParRed.phi
+      apply ParRed.refl; apply ParRed.refl; apply ParRed.refl
+    }
+    case bind1 t1 t1' k t2 _ ih => {
+      apply ParRed.bind; exact ih
+      intro x _; apply ParRed.refl; exact []
+    }
+    case bind2 t2 t2' k t1 S _ ih => {
+      apply ParRed.bind; apply ParRed.refl; exact ih
+    }
+    case ctor1 t1 t1' k t2 t3 _ ih => {
+      apply ParRed.ctor; exact ih
+      apply ParRed.refl; apply ParRed.refl
+    }
+    case ctor2 t2 t2' k t1 t3 _ ih => {
+      apply ParRed.ctor; apply ParRed.refl
+      exact ih; apply ParRed.refl
+    }
+    case ctor3 t3 t3' k t1 t2 _ ih => {
+      apply ParRed.ctor; apply ParRed.refl
+      apply ParRed.refl; exact ih
+    }
+  }
+
+  lemma red_implies_par : t -β>* s -> t -p>* s := by {
+    intro step
+    induction step
+    case refl => apply ParRedStar.refl
+    case step t1 t2 t3 r1 _r2 ih => {
+      have lem := red_implies_par_step r1
+      apply ParRedStar.step lem ih
+    }
+  }
+
+  lemma par_implies_red_step : t -p> s -> t -β>* s := by {
+    intro step
+    induction step
+    case beta t1 t1' t2 t2' t3 t3' m S h1 ih1 h2 ih2 h3 ih3 => {
+      have r1 : app m (lam m t1 t2) t3 -β>* app m (lam m t1 t2') t3' := by {
+        have xfresh := @Name.fresh_is_fresh (S ++ fv t2 ++ fv t2')
+        generalize xdef : @Name.fresh (S ++ fv t2 ++ fv t2') = x at *
+        simp at *; replace xfresh := demorgan3 xfresh
+        casesm* _ ∧ _; case _ xn1 xn2 xn3 =>
+        apply red_ctor
+        apply red_bind2 x
+        simp [*]
+        apply h3 x xn1; apply ih3; apply RedStar.refl
+      }
+      have r2 := RedStar.step (@Red.beta m t1 t2' t3') RedStar.refl
+      apply RedStar.trans r1 r2
+    }
+    case fst t1 t1' t2 t2' t3 t3' h1 h2 h3 ih1 ih2 ih3 => {
+      have r1 : fst (pair t1 t2 t3) -β>* fst (pair t1' t2 t3) := by {
+        sorry
+      }
+      have r2 := RedStar.step (@Red.fst t1' t2 t3) RedStar.refl
+      apply RedStar.trans r1 r2
+    }
+    case snd => sorry
+    case eqind => sorry
+    case promote => sorry
+    case phi => sorry
+    case bind t1 t1' t2 t2' k S s1 ih1 s2 ih2 => {
+      have xfresh := @Name.fresh_is_fresh (S ++ fv t2 ++ fv t2')
+      generalize xdef : @Name.fresh (S ++ fv t2 ++ fv t2') = x at *
+      simp at *; replace xfresh := demorgan3 xfresh
+      casesm* _ ∧ _; case _ xn1 xn2 xn3 =>
+      apply red_bind x
+      apply s2
+      simp [*]
+      apply ih2 x xn1
+    }
+    case ctor t1 t1' t2 t2' t3 t3' k h1 h2 h3 ih1 ih2 ih3 => {
+      apply red_ctor ih1 ih2 ih3
+    }
+    case const => apply RedStar.refl
+    case free => apply RedStar.refl
+    case bound i => cases i; linarith
+  }
+
+  lemma par_implies_red : t -p>* s -> t -β>* s := by {
+    intro step
+    induction step
+    case refl => apply RedStar.refl
+    case step t1 t2 t3 r1 _r2 ih => {
+      have lem := par_implies_red_step r1
+      apply RedStar.trans lem ih
+    }
+  }
+
+  @[simp] lemma parp_kindu {n} : parp kindu = @kindu n := by {
+    unfold parp; unfold kindu; simp
+  }
+
+  lemma parp_open {n} (t : Term (n + 1)) : {_|-> x}parp t = parp ({_|-> x}t) := by {
+    sorry
+  }
+
+  lemma par_subst (S : FvSet!) :
+    t -p> t' ->
+    (∀ x, x ∉ S -> {_|-> x}s -p> {_|-> x}s') ->
+    [_:= t]s -p> [_:= t']s'
+  := by {
+    intro r1 r2
+    have xfresh := @Name.fresh_is_fresh (S ++ fv s ++ fv s')
+    generalize xdef : @Name.fresh (S ++ fv s ++ fv s') = x at *
+    simp at xfresh; replace xfresh := demorgan3 xfresh
+    casesm* _ ∧ _; case _ xn1 xn2 xn3 =>
+    have r3 := r2 x xn1
+    generalize zdef : {_|-> x}s = z at *
+    generalize zpdef : {_|-> x}s' = z' at *
+    induction r3 generalizing t t' s s'
+    case beta t1 t1' t2 t2' t3 t3' m S' h1 h2 h3 ih1 ih2 ih3 => {
+      replace zdef := open_to_close xn2 zdef; simp at zdef
+      replace zpdef := open_to_close xn3 zpdef
+      subst zdef; subst zpdef; simp
+      rw [subst_hsubst_commute]
+      apply ParRed.beta; apply ParRed.refl
+      repeat sorry
+    }
+    case fst t1 t1' t2 t2' t3 t3' h1 h2 h3 ih1 ih2 ih3 => {
+      replace zdef := open_to_close xn2 zdef; simp at zdef
+      replace zpdef := open_to_close xn3 zpdef; simp at zpdef
+      subst zdef; subst zpdef; simp
+      sorry
+    }
+    case snd => sorry
+    case eqind => sorry
+    case promote => sorry
+    case phi => sorry
+    case bind => sorry
+    case ctor => sorry
+    case const => sorry
+    case free => sorry
+    case bound => sorry
+  }
+
+  lemma par_triangle : t -p> s -> s -p> (parp t) := by {
+    intro step
+    induction step
+    case beta t1 t1' t2 t2' t3 t3' m S h1 h2 h3 ih1 ih2 ih3 => {
+      unfold app; unfold lam; unfold parp; unfold kindu; simp
+      have lem : ∀ x ∉ S, {_|-> x}t2' -p> {_|-> x}(parp t2) := by {
+        intro x xn; rw [parp_open]
+        apply ih2 x xn
+      }
+      apply par_subst S ih3 lem
+    }
+    case fst t1 t1' t2 t2' t3 t3' h1 h2 h3 ih1 ih2 ih3 => exact ih1
+    case snd t1 t1' t2 t2' t3 t3' h1 h2 h3 ih1 ih2 ih3 => exact ih2
+    case eqind t1 t1' t2 t2' t3 t3' t4 t4' t5 t5' t6 t6'
+      h1 h2 h3 h4 h5 h6 ih1 ih2 ih3 ih4 ih5 ih6 =>
+    {
+      apply ParRed.ctor; exact ih6; exact ih5
+      apply ParRed.refl
+    }
+    case promote t t' h ih => {
+      apply ParRed.ctor; exact ih
+      apply ParRed.refl; apply ParRed.refl
+    }
+    case phi t1 t1' t2 t2' t3 t3' h1 h2 h3 ih1 ih2 ih3 => exact ih1
+    case bind t1 t1' t2 t2' k S h1 h2 ih1 ih2 => {
+      cases k <;> simp
+      case lam m => {
+        sorry
+      }
+      case pi m => sorry
+      case inter => sorry
+    }
+    case ctor t1 t1' t2 t2' t3 t3' k h1 h2 h3 ih1 ih2 ih3 => {
+      cases k
+      case app => sorry
+      case pair => {
+        unfold parp; simp
+        apply ParRed.ctor; apply ih1; apply ih2; apply ih3
+      }
+      case fst => {
+        generalize H : (parp (Syntax.ctor Constructor.fst t1 t2 t3)) = t
+        unfold parp at H
+        split at H
+        all_goals injections
+        case _ t' u1 u2 u3 e1 e2 e3 e4 => {
+          subst e2; subst e3; subst e4; simp at *
+          cases h2; case _ =>
+          cases h3; case _ =>
+          simp at *
+          unfold pair at ih1; unfold parp at ih1
+          cases t1' <;> try cases ih1
+          case ctor k v1 v2 v3 => {
+            cases k <;> try cases h1
+            case _ h1 h2 h3 => {
+              cases ih1; case _ h4 h5 h6 =>
+              simp; rw [<-H]; apply ParRed.fst
+              apply h4; apply h5; apply h6
+            }
+          }
+        }
+        case _ => sorry
+        case _ t' k u1 u2 u3 m1 m2 m3 m4 m5 h e1 e2 e3 e4 e5 => {
+          subst e2; subst e3; subst e4; subst e5; simp at *
+          rw [<-H]; apply ParRed.ctor; exact ih1; exact ih2; exact ih3
+        }
+      }
+      case snd => sorry
+      case eq => sorry
+      case refl => sorry
+      case eqind => sorry
+      case j0 => sorry
+      case jω => sorry
+      case promote => sorry
+      case delta => sorry
+      case phi => sorry
+    }
+    case const => unfold parp; unfold const; simp; apply ParRed.refl
+    case free => unfold parp; unfold free; simp; apply ParRed.refl
+    case bound i => cases i; linarith
+  }
+
+  lemma par_diamond : t -p> t1 -> t -p> t2 -> ∃ k, t1 -p> k ∧ t2 -p> k := by {
+    intro r1 r2
+    exists (parp t)
+    apply And.intro _ _
+    apply par_triangle r1
+    apply par_triangle r2
+  }
+
+  lemma par_strip : t -p> t1 -> t -p>* t2 -> ∃ z, t1 -p>* z ∧ t2 -p> z := by {
+    intro r1 r2
+    induction r2 generalizing t1
+    case refl t' => {
+      exists t1; apply And.intro _ _
+      apply ParRedStar.refl; apply r1
+    }
+    case step u1 u2 u3 s1 _s2 ih => {
+      have lem := par_triangle s1
+      replace ih := ih lem
+      have lem2 := par_triangle r1
+      casesm* ∃ _, _, _ ∧ _; case _ z rr1 rr2 =>
+      exists z; apply And.intro _ rr2
+      apply ParRedStar.step lem2 rr1
+    }
+  }
+
+  lemma par_confluence : t -p>* t1 -> t -p>* t2 -> ∃ z, t1 -p>* z ∧ t2 -p>* z := by {
+    intro r1 r2
+    induction r1 generalizing t2
+    case refl t' => {
+      exists t2; apply And.intro r2 _
+      apply ParRedStar.refl
+    }
+    case step u1 u2 u3 s1 _s2 ih => {
+      have lem1 := par_strip s1 r2
+      casesm* ∃ _, _, _ ∧ _; case _ z1 rr1 rr2 =>
+      replace ih := ih rr1
+      casesm* ∃ _, _, _ ∧ _; case _ z2 rr3 rr4 =>
+      exists z2; apply And.intro rr3
+      apply ParRedStar.step rr2 rr4
+    }
+  }
+
+  theorem confluence : t -β>* t1 -> t -β>* t2 -> ∃ z, t1 -β>* z ∧ t2 -β>* z := by {
+    intro r1 r2
+    have p1 := red_implies_par r1
+    have p2 := red_implies_par r2
+    have lem := par_confluence p1 p2
+    casesm* ∃ _, _, _ ∧ _; case _ z p3 p4 =>
+    have r3 := par_implies_red p3
+    have r4 := par_implies_red p4
+    exists z
+  }
 
 end Cedille
