Cedille/Lemma/Preservation.lean
@@ -6,441 +6,291 @@ import Cedille.Lemma.Refold
 import Cedille.Lemma.Erasure
 import Cedille.Lemma.Inversion
 import Cedille.Lemma.Red
+import Cedille.Lemma.Conv
+import Cedille.Lemma.Rule
 
 namespace Cedille
 
-  lemma preservation_of_infer_step_subst :
-    Γ ⊢ lam m u1 u2 >: pi m A B ->
-    Γ ⊢ u3 =: A ->
-    ∃ B, Γ ⊢ [_:= u3]u2 : B
-  := by sorry
+  inductive CtxRed : (Map! (Term 0)) -> (Map! (Term 0)) -> Prop where
+  | head (x:Name) A : CtxRed Γ Δ -> CtxRed (Γ ++ [x:A]) (Δ ++ [x:A])
+  | tail (x:Name) Γ : A -β> B -> CtxRed (Γ ++ [x:A]) (Γ ++ [x:B])
 
-  lemma preservation_step_of_infer_ctx (S : FvSet!) :
-    ((x : Name) -> x ∉ S → (Γ ++ [x:A]) ⊢ {_|-> x}t : {_|-> x}B) ->
-    A -β> A' ->
-    ∃ B, ((x : Name) -> x ∉ S → (Γ ++ [x:A']) ⊢ {_|-> x}t : {_|-> x}B)
-  := by sorry
+  -- lemma preservation_of_proof :
+  --   Γ ⊢ t : A ->
+  --   (∀ t', t -β> t' -> ∃ A', A -β>* A' ∧ Γ ⊢ t' : A')
+  --   ∧ (∀ Γ', CtxRed Γ Γ' -> ∃ A', A -β>* A' ∧ Γ' ⊢ t : A')
+  -- := λ j => @Infer.rec
+  --   (λ Γ t A j =>
+  --     (∀ t', t -β> t' -> ∃ A', A -β>* A' ∧ Γ ⊢ t' : A')
+  --     ∧ (∀ Γ', CtxRed Γ Γ' -> ∃ A', A -β>* A' ∧ Γ' ⊢ t : A'))
+  --   (λ Γ t A j =>
+  --     (∀ t', t -β> t' -> ∃ A', A -β>* A' ∧ Γ ⊢ t' : A')
+  --     ∧ (∀ Γ', CtxRed Γ Γ' -> ∃ A', A -β>* A' ∧ Γ' ⊢ t : A'))
+  --   (λ Γ t A j =>
+  --     (∀ t', t -β> t' -> ∃ A', A -β>* A' ∧ Γ ⊢ t' : A')
+  --     ∧ (∀ Γ', CtxRed Γ Γ' -> ∃ A', A -β>* A' ∧ Γ' ⊢ t : A'))
+  --   (λ Γ wf => ∀ Γ', CtxRed Γ Γ' -> ⊢ Γ')
+  --   sorry
+  --   sorry
+  --   sorry
+  --   sorry
+  --   sorry
+  --   sorry
+  --   sorry
+  --   sorry
+  --   sorry
+  --   sorry
+  --   sorry
+  --   sorry
+  --   sorry
+  --   sorry
+  --   sorry
+  --   sorry
+  --   (by {
+  --     intro Γ t A B K j1 j2 j3 ih1 ih2
+  --     sorry
+  --   })
+  --   sorry
+  --   sorry
+  --   Γ
+  --   t
+  --   A
+  --   j
 
-  lemma preservation_step_of_cinfer_ctx (S : FvSet!) :
-    ((x : Name) -> x ∉ S → (Γ ++ [x:A]) ⊢ {_|-> x}t >: {_|-> x}B) ->
-    A -β> A' ->
-    ((x : Name) -> x ∉ S → (Γ ++ [x:A']) ⊢ {_|-> x}t >: {_|-> x}B)
-  := by sorry
 
-  lemma preservation_step_of_cinfer_ctx_const (S : FvSet!) :
-    ((x : Name) -> x ∉ S → (Γ ++ [x:A]) ⊢ {_|-> x}t >: const K) ->
-    A -β> A' ->
-    ((x : Name) -> x ∉ S → (Γ ++ [x:A']) ⊢ {_|-> x}t >: const K)
-  := by sorry
 
-  lemma rule_cinfer_red : Γ ⊢ t >: A -> A -β>* B -> Γ ⊢ t >: B := by {
-    intro j step
-    cases j; case _ D j step2 =>
-    replace step := RedStar.trans step2 step
-    apply ConInfer.infer j step
-  }
+  -- lemma preservation_of_cinfr :
+  --   Γ ⊢ A >: typeu ->
+  --   (∀ B, A -β> B -> Γ ⊢ B >: typeu) ∧ (∀ Δ, CtxRed Γ Δ -> Δ ⊢ A >: typeu)
+  -- := λ j => @ConInfer.rec
+  --   (λ Γ A K j => K = typeu -> (∀ B, A -β> B -> Γ ⊢ B : K) ∧ (∀ Δ, CtxRed Γ Δ -> Δ ⊢ A : K))
+  --   (λ Γ A K j => K = typeu -> (∀ B, A -β> B -> Γ ⊢ B >: K) ∧ (∀ Δ, CtxRed Γ Δ -> Δ ⊢ A >: K))
+  --   (λ Γ A K j => (∀ B, A -β> B -> Γ ⊢ B =: K) ∧ (∀ Δ, CtxRed Γ Δ -> Δ ⊢ A =: K))
+  --   (λ Γ j => ∀ Δ, CtxRed Γ Δ -> ⊢ Δ)
+  --   (by {
+  --     intro Γ wf ih eq
+  --     sorry -- EASY
+  --   })
+  --   (by {
+  --     intro Γ x A wf xin ih eq
+  --     apply And.intro _ _
+  --     intro B step; cases step
+  --     intro Δ step; replace ih := ih Δ step
+  --     sorry -- EASY
+  --   })
+  --   (by {
+  --     intro Γ A m K C S j1 j2 ih1 ih2 eq; simp at *
+  --     sorry
+  --   })
+  --   (by {
+  --     intro Γ A m K t B S j1 j2 j3 ih1 ih2 eq
+  --     sorry
+  --   })
+  --   (by {
+  --     intro Γ f m A B a S j1 j2 ih1 ih2
+  --     sorry
+  --   })
+  --   sorry
+  --   sorry
+  --   sorry
+  --   sorry
+  --   (by {
+  --     intro Γ A a b j1 j2 j3 ih1 ih2 ih3 _
+  --     apply And.intro _ _
+  --     intro B step
+  --     cases step
+  --     case ctor1 => sorry
+  --     case ctor2 => sorry
+  --     case ctor3 _ b' step => {
+  --       simp at *
+  --       sorry
+  --     }
+  --     sorry
+  --   })
+  --   sorry
+  --   sorry
+  --   sorry
+  --   sorry
+  --   sorry
+  --   (by {
+  --     intro Γ t A B j1 j2 ih
+  --     sorry
+  --   })
+  --   (by {
+  --     intro Γ t A B K j1 j2 j3 ih1 ih2
+  --     apply And.intro _ _
+  --     intro t' step
+  --     sorry
+  --     sorry
+  --   })
+  --   sorry
+  --   sorry
+  --   Γ
+  --   A
+  --   typeu
+  --   j
+  --   (by simp)
 
-  lemma rule_inv_inter1_kind : ¬ (Γ ⊢ t >: inter (const K) B) := λ j => @Nat.rec
-    (λ s => ∀ Γ t K B,
-      size t ≤ s ->
-      ¬ Γ ⊢ t >: inter (const K) B)
+  lemma preservation :
+    Γ ⊢ t >: A ->
+    (∀ s, t -β> s -> Γ ⊢ s >: A)
+    ∧ (∀ B, A -β>* B -> Γ ⊢ t >: B)
+    ∧ (∀ Δ, CtxRed Γ Δ -> Δ ⊢ t >: A)
+  := λ j => @ConInfer.rec
+    (λ Γ t A j => (∀ s, t -β> s -> Γ ⊢ s >: A)
+      ∧ (∀ B, A -β>* B -> Γ ⊢ t >: B)
+      ∧ (∀ Δ, CtxRed Γ Δ -> Δ ⊢ t >: A))
+    (λ Γ t A j => (∀ s, t -β> s -> Γ ⊢ s >: A)
+      ∧ (∀ B, A -β>* B -> Γ ⊢ t >: B)
+      ∧ (∀ Δ, CtxRed Γ Δ -> Δ ⊢ t >: A))
+    (λ Γ t A j => (∀ s, t -β> s -> Γ ⊢ s =: A)
+      ∧ (∀ B, A -β>* B -> Γ ⊢ t =: B)
+      ∧ (∀ Δ, CtxRed Γ Δ -> Δ ⊢ t =: A))
+    (λ Γ j => ∀ Δ, CtxRed Γ Δ -> ⊢ Δ)
+    (by {
+      sorry
+    })
+    (by {
+      sorry
+    })
+    (by {
+      sorry
+    })
+    (by {
+      sorry
+    })
+    (by {
+      intro Γ f m A B a S j1 j2 ih1 ih2
+      sorry
+    })
     sorry
     (by {
-      intro s ih Γ t K B sh j
-      cases t <;> simp at *
-      case bound => apply ih _ (bound _) _ _ (by simp) j
-      case free => apply ih _ (free _) _ _ (by simp) j
-      case const => apply ih _ (const _) _ _ (by simp) j
-      case bind b u1 u2 => {
-        cases b <;> simp at *
-        case lam m => {
+      intro Γ T A B t s S j1 j2 j3 j4 ih1 ih2 ih3
+      casesm* _ ∧ _; case _ ih1 ih2 ih3 ih4 ih5 ih6 ih7 ih8 ih9 =>
+      apply And.intro _ _
+      {
+        intro q step
+        cases step <;> simp
+        case ctor1 t' step => {
+          constructor; constructor; exact S
+          exact j1; apply ih2 t' step
+          have lem : [_:= t]B -β>* [_:= t']B := sorry
+          repeat sorry
+        }
+        case ctor2 => sorry
+        case ctor3 => sorry
+      }
+      apply And.intro _ _
+      {
+        intro Q step
+        sorry
+        -- cases step <;> simp
+        -- case bind1 A' step => {
+        --   constructor; constructor; exact S
+        --   exact j1; exact j2; exact j3; exact j4
+        --   apply red_bind1 (RedStar.step step RedStar.refl)
+        -- }
+        -- case bind2 B' S' step => {
+        --   constructor; constructor; exact (S ++ S')
+        --   exact j1; exact j2; exact j3; exact j4
+        --   have xfresh := @Name.fresh_is_fresh (S ++ S' ++ fv B ++ fv B')
+        --   generalize xdef : @Name.fresh (S ++ S' ++ fv B ++ fv B') = x at *
+        --   simp at *
+        --   replace xfresh := demorgan4 xfresh
+        --   casesm* _ ∧ _; case _ xn1 xn2 xn3 xn4 =>
+        --   have xn5 : x ∉ (fv B ++ fv B') := by simp [*]
+        --   have step2 := RedStar.step (step x xn2) RedStar.refl
+        --   apply red_bind2 x xn5 step2
+        -- }
+      }
+      intro Δ step
+      constructor; constructor; exact S
+      apply ih5 Δ step; apply ih7 Δ step; apply ih9 Δ step; exact j4
+      apply RedStar.refl
+    })
+    sorry
+    sorry
+    (by {
+      intro Γ A a b j1 j2 j3 ih1 ih2 ih3
+      casesm* _ ∧ _; case _ ih1 ih2 ih3 ih4 ih5 ih6 ih7 ih8 ih9 =>
+      apply And.intro _ _
+      {
+        intro s step
+        cases step <;> simp
+        case ctor1 A' step => {
+          have steps := RedStar.step step RedStar.refl
+          constructor; constructor
+          apply ih1 A' step; apply ih6 A' steps; apply ih8 A' steps
+          apply RedStar.refl
+        }
+        case ctor2 a' step => {
+          constructor; constructor
+          apply j1; apply ih2 a' step; apply j3
+          apply RedStar.refl
+        }
+        case ctor3 b' step => {
+          constructor; constructor
+          apply j1; apply j2; apply ih3 b' step
+          apply RedStar.refl
+        }
+      }
+      apply And.intro _ _
+      {
+        intro B' step
+        cases step
+        case refl => {
+          constructor; constructor
+          exact j1; exact j2; exact j3; exact RedStar.refl
+        }
+        case step _ step _ => cases step
+      }
+      intro Δ step
+      constructor; constructor
+      apply ih5 Δ step; apply ih7 Δ step; apply ih9 Δ step
+      apply RedStar.refl
+    })
+    sorry
+    sorry
+    sorry
+    sorry
+    sorry
+    (by {
+      intro Γ t A B j1 j2 ih
+      sorry
+    })
+    (by {
+      intro Γ t A B K j1 j2 j3 ih1 ih2
+      casesm* _ ∧ _; case _ ih1 ih2 ih3 ih4 ih5 ih6 => {
+        apply And.intro _ _
+        {
+          intro s step
+          replace ih1 := ih1 s step
+          cases ih1; case _ T j step2 =>
+          constructor; exact j; exact j2
+          apply Conv.red_b j3 step2
+        }
+        apply And.intro _ _
+        {
           sorry
+          -- intro B' step
+          -- replace ih2 := ih2 B' step
+          -- constructor; exact j1; exact ih2
+          -- have lem : A === B' := by {
+          --   have lem1 := Conv.symm j3
+          --   cases j2; case _ j2 _ =>
+          --   have h := infer_implies_sane j2
+          --   have lem2 := Conv.red_f h lem1 (RedStar.step step RedStar.refl)
+          --   apply Conv.symm lem2
+          -- }
+          -- exact lem
         }
-        case pi m => sorry
-        case inter => sorry
+        intro Δ step
+        replace ih6 := ih6 Δ step
+        replace ih4 := ih4 Δ step
+        cases ih4; case _ T j step2 =>
+        constructor; exact j; exact ih6
+        apply Conv.red_b j3 step2
       }
-      case ctor => sorry
-    })
-    (size t)
-    Γ
-    t
-    K
-    B
-    (by simp)
-    j
-
-  lemma preservation_step_of_cinfer_const :
-    Γ ⊢ t >: const K ->
-    t -β> s ->
-    Γ ⊢ s >: const K
-  := λ j step => @ConInfer.rec
-    (λ Γ t A j => ∀ s K, A -β>* const K -> t -β> s -> Γ ⊢ s : A)
-    (λ Γ t A j => ∀ s K, A = const K -> t -β> s -> Γ ⊢ s >: A)
-    (λ Γ t A j => ∀ s K, A = const K -> t -β> s -> Γ ⊢ s =: A)
-    (λ Γ wf => True)
-    (by {
-      intro Γ wf _ s K e step
-      cases step
-    })
-    (by {
-      intro Γ x A wf xn _ s K e step
-      cases step
-    })
-    (by {
-      intro Γ A m K B S j1 j2 ih1 ih2 s K' e step; simp at *
-      cases step <;> simp at *
-      case bind1 A' step => {
-        cases m <;> simp at *
-        case free => {
-          have lem1 := ih1 A' Constant.typeU rfl step
-          have lem2 := preservation_step_of_cinfer_ctx_const S j2 step
-          apply @Infer.pi _ _ mf Constant.typeU _ _ lem1 lem2
-        }
-        case erased => {
-          have lem1 := ih1 A' K rfl step
-          have lem2 := preservation_step_of_cinfer_ctx_const S j2 step
-          apply @Infer.pi _ _ m0 K _ _ lem1 lem2
-        }
-        case type => {
-          have lem1 := ih1 A' K rfl step
-          have lem2 := preservation_step_of_cinfer_ctx_const S j2 step
-          apply @Infer.pi _ _ mt K _ _ lem1 lem2
-        }
-      }
-      case bind2 B' S' step => {
-        cases m <;> simp at *
-        case free => {
-          have lem2 : ∀ x, x ∉ (S ++ S') -> (Γ ++ [x:A]) ⊢ {_|-> x}B' >: typeu := by {
-            intro x xn; simp at xn
-            replace xn := demorgan xn
-            cases xn; case _ xn1 xn2 =>
-            apply ih2 x xn1 ({_|-> x}B') Constant.typeU rfl _
-            apply step x xn2
-          }
-          apply @Infer.pi _ _ mf Constant.typeU _ (S ++ S') j1 lem2
-        }
-        case erased => {
-          have lem2 : ∀ x, x ∉ (S ++ S') -> (Γ ++ [x:A]) ⊢ {_|-> x}B' >: typeu := by {
-            intro x xn; simp at xn
-            replace xn := demorgan xn
-            cases xn; case _ xn1 xn2 =>
-            apply ih2 x xn1 ({_|-> x}B') Constant.typeU rfl _
-            apply step x xn2
-          }
-          apply @Infer.pi _ _ m0 K _ (S ++ S') j1 lem2
-        }
-        case type => {
-          have lem2 : ∀ x, x ∉ (S ++ S') -> (Γ ++ [x:A]) ⊢ {_|-> x}B' >: kindu := by {
-            intro x xn; simp at xn
-            replace xn := demorgan xn
-            cases xn; case _ xn1 xn2 =>
-            apply ih2 x xn1 ({_|-> x}B') Constant.kindU rfl _
-            apply step x xn2
-          }
-          apply @Infer.pi _ _ mt K _ (S ++ S') j1 lem2
-        }
-      }
-    })
-    sorry
-    sorry
-    sorry
-    (sorry)
-    (by {
-      intro Γ t A B j ih s K e step
-      sorry
-    })
-    sorry
-    (by {
-      intro Γ A a b j1 j2 j3 ih1 ih2 ih3 s K e step
-      cases step <;> simp at *
-      case ctor1 => sorry
-      case ctor2 a' step => {
-        sorry
-      }
-      case ctor3 => sorry
-    })
-    sorry
-    sorry
-    sorry
-    sorry
-    sorry
-    (by {
-      intro Γ t A B j step ih s K e step'
-      subst e
-      have lem := ih s K step step'
-      apply ConInfer.infer lem step
-    })
-    (by {
-      intro Γ t A B K' j1 j2 conv ih1 ih2 s K e step
-      subst e;
-      cases conv; case _ A' K' S s1 er s2 =>
-      cases s2
-      case refl => {
-        clear ih2
-        sorry
-      }
-      case step _ step _ => cases step
-    })
-    (by simp)
-    (by simp)
-    Γ
-    t
-    (const K)
-    j
-    s
-    K
-    rfl
-    step
-
-
-  lemma preservation_step_of_cinfer_pi_domain :
-    Γ ⊢ t >: Mode.pi_domain m K ->
-    t -β> s ->
-    Γ ⊢ s >: Mode.pi_domain m K
-  := λ j step => @Nat.rec
-    (λ si => ∀ Γ t m K s,
-      size t ≤ si ->
-      Γ ⊢ t >: Mode.pi_domain m K ->
-      t -β> s ->
-      Γ ⊢ s >: Mode.pi_domain m K)
-    sorry
-    (by {
-      intro si ih Γ t m K s sh j step
-      cases t <;> simp at *
-      case bound => cases step
-      case free => cases step
-      case const => cases step
-      case bind b u1 u2 => {
-        have s1 : size u1 ≤ si := by linarith 
-        have s2 : size u2 ≤ si := by linarith
-        cases b <;> simp at *
-        case lam m' => {
-          cases j; case _ D j step2 =>
-          cases j; case _ K2 B2 S2 j1 j2 j3 =>
-          exfalso; apply red_inv_pi_not_pi_domain step2
-        }
-        case pi m' => {
-          cases j; case _ D j step2 =>
-          cases j; case _ K2 S2 j1 j2 =>
-          have e := red_force_mode_pi_codomain step2; rw [e]
-          cases step <;> simp
-          case bind1 u1' step => {
-            cases m' <;> simp at *
-            case free => {
-              have lem := @ih Γ u1 mf Constant.typeU u1' s1 j1 step; simp at lem
-              apply ConInfer.infer _ _; exact typeu
-              apply @Infer.pi _ _ mf Constant.typeU _ S2 lem
-              simp; apply preservation_step_of_cinfer_ctx_const S2 j2 step
-              apply RedStar.refl
-            }
-            case erased => sorry
-            case type => sorry
-          }
-          case bind2 => sorry
-        }
-        case inter => {
-          cases j; case _ D j step2 =>
-          cases j; case _ S2 j1 j2 =>
-          have e := red_force_typeu step2; rw [e]
-          cases step <;> simp
-          case bind1 u1' step => {
-            have lem := @ih Γ u1 mf K u1' s1 j1 step; simp at lem
-            sorry
-          }
-          case bind2 => sorry
-        }
-      }
-      case ctor c u1 u2 u3 => {
-        have s1 : size u1 ≤ si := by linarith 
-        have s2 : size u2 ≤ si := by linarith
-        have s3 : size u3 ≤ si := by linarith
-        cases c <;> simp at *
-        case app m => sorry
-        case pair => {
-          cases j; case _ D j step2 =>
-          cases j; case _ A B j1 j2 j3 j4 =>
-          exfalso; apply red_inv_inter_not_pi_domain step2
-        }
-        case fst => {
-          cases j; case _ D j step2 =>
-          cases j; case _ B j =>
-          have step2 : inter D B -β>* inter (Mode.pi_domain m K) B := by {
-            apply red_inter' step2 (λ _ _ => RedStar.refl); exact []
-          }
-          replace j := rule_cinfer_red j step2
-          cases m <;> simp at *
-          case free => exfalso; apply rule_inv_inter1_kind j
-          case erased => exfalso; apply rule_inv_inter1_kind j
-          case type => exfalso; apply rule_inv_inter1_kind j
-        }
-        case snd => sorry
-        case eq => sorry
-        case refl => sorry
-        case eqind => sorry
-        case j0 => sorry
-        case jω => sorry
-        case promote => sorry
-        case delta => sorry
-        case phi => sorry
-      }
-    })
-    (size t)
-    Γ
-    t
-    m
-    K
-    s
-    (by simp)
-    j
-    step
-
-
-  lemma preservation_of_infer_step4 : Γ ⊢ t : A -> t -β> s -> Γ ⊢ s : A := by {
-    intro j step
-    induction step generalizing Γ A
-    case beta m u1 u2 u3 => {
-      cases j; case _ A B S j1 j2 =>
-      sorry
-    }
-    case fst u1 u2 u3 => {
-      cases j; case _ B j =>
-      cases j; case _ T j step =>
-      sorry
-    }
-    case snd => sorry
-    case eqind => sorry
-    case promote => sorry
-    case phi => sorry
-    case bind1 => sorry
-    case bind2 => sorry
-    case ctor1 => sorry
-    case ctor2 => sorry
-    case ctor3 => sorry
-  }
-
-  lemma preservation_of_infer_step : Γ ⊢ t : A -> t -β> s -> ∃ B, Γ ⊢ s : B := by {
-    intro tproof step
-    induction step generalizing Γ A
-    case beta m u1 u2 u3 => {
-      cases tproof; case _ A B S j1 j2 =>
-      apply preservation_of_infer_step_subst j1 j2
-    }
-    case fst u1 u2 u3 => {
-      cases tproof; case _ B j =>
-      cases j; case _ P j step =>
-      cases j; case _ A2 B2 j1 j2 j3 j4 =>
-      cases j1; case _ A3 j5 j6 =>
-      sorry
-    }
-    case snd u1 u2 u3 => {
-      cases tproof; case _ A1 B1 j =>
-      cases j; case _ P j1 s1 =>
-      cases j1; case _ A2 B2 j1 j2 j3 j4 =>
-      cases j3; case _ A3 j5 c1 =>
-      sorry
-    }
-    case eqind u1 u2 u3 u4 u5 u6 => {
-      cases tproof
-      case eqind j1 j2 j3 j4 j5 j6 => {
-        cases j5; case _ D j5 c1 =>
-        cases j5; case _ A j =>
-        sorry
-      }
-    }
-    case promote u => {
-      cases tproof; case _ T a b A B j1 j2 =>
-      cases j2; case _ A2 j2 s1 =>
-      cases j2; case _ A3 j2 =>
-      cases j2; case _ B2 j2 =>
-      cases j2; case _ T j s2 =>
-      exists eq T u u
-      apply Infer.refl; simp [*]
-    }
-    case phi => sorry
-    case bind1 u1 u2 k u3 s1 ih => {
-      cases k <;> simp at *
-      case lam m => {
-        cases tproof; case _ K B S j1 j2 j3 =>
-        cases j1; case _ T j1 step2 =>
-        have lem := ih j1
-        cases lem; case _ D jlem =>
-        have cj1 : Γ ⊢ u1 >: Mode.pi_domain m K := ConInfer.infer j1 step2
-        have lem1 := preservation_step_of_cinfer_pi_domain cj1 s1
-        have lem2 := @preservation_step_of_infer_ctx Γ u1 u3 B u2 S j3 s1
-        cases lem2; case _ B' lem2 =>
-        exists (pi m u2 B')
-        apply Infer.lam lem1 lem2 j2
-      }
-      case pi m => sorry
-      case inter => sorry
-    }
-    case bind2 u1 u2 k u3 S1 s1 ih => {
-      cases k <;> simp at *
-      case lam m => {
-        cases tproof; case _ K B S2 j1 j2 j3 =>
-        have xfresh := @Name.fresh_is_fresh (S1 ++ S2)
-        generalize xdef : Name.fresh (S1 ++ S2) = x at *
-        simp at *
-        replace xfresh := demorgan xfresh
-        cases xfresh; case _ xn1 xn2 =>
-        have lem1 := ih x xn1 (j3 x xn2)
-        cases lem1; case _ D lem1 =>
-        have lem2 := to_open D x
-        cases lem2; case _ D' lem2 =>
-        subst lem2
-        exists pi m u3 D'
-        apply Infer.lam j1 _ _
-        exact S2; intro y yn
-        sorry
-
-
-        sorry
-      }
-      case pi m => sorry
-      case inter => sorry
-    }
-    case ctor1 => sorry
-    case ctor2 => sorry
-    case ctor3 => sorry
-  }
-
-  lemma preservation_of_infer_step3 : Γ ⊢ t : A -> t -β> s -> ∃ B, Γ ⊢ s : B
-    := λ j step => @Infer.rec
-      (λ Γ t A j' => ∀ s, t -β> s -> ∃ B, Γ ⊢ s : B)
-      (λ Γ t A j' => ∀ s, t -β> s -> ∃ B, Γ ⊢ s >: B)
-      (λ Γ t A j' => ∀ s, t -β> s -> ∃ B, Γ ⊢ s =: B)
-      (λ Γ wf => True)
-    sorry
-    sorry
-    sorry
-    (by {
-      intro Γ A m K t B S j1 j2 j3 ih1 ih2 s step; simp at *
-      cases step <;> simp
-      case bind1 A' step => {
-        sorry
-      }
-      case bind2 => sorry
-    })
-    sorry
-    sorry
-    sorry
-    sorry
-    sorry
-    sorry
-    sorry
-    sorry
-    sorry
-    sorry
-    sorry
-    (by {
-      intro Γ t A B j step ih s step2
-      have lem := ih s step2
-      cases lem; case _ D j2 =>
-      sorry
-    })
-    (by {
-      intro Γ t A B j c ih s step
-      sorry
     })
     sorry
     sorry
@@ -448,9 +298,450 @@ namespace Cedille
     t
     A
     j
-    s
-    step
 
-  theorem preservation_of_infer : Γ ⊢ t : A -> t -β>* s -> ∃ B, Γ ⊢ s : B := sorry 
+
+  -- lemma preservation_of_infer_step_subst :
+  --   Γ ⊢ lam m u1 u2 >: pi m A B ->
+  --   Γ ⊢ u3 =: A ->
+  --   ∃ B, Γ ⊢ [_:= u3]u2 : B
+  -- := by sorry
+
+  -- lemma preservation_step_of_infer_ctx (S : FvSet!) :
+  --   ((x : Name) -> x ∉ S → (Γ ++ [x:A]) ⊢ {_|-> x}t : {_|-> x}B) ->
+  --   A -β> A' ->
+  --   ∃ B, ((x : Name) -> x ∉ S → (Γ ++ [x:A']) ⊢ {_|-> x}t : {_|-> x}B)
+  -- := by sorry
+
+  -- lemma preservation_step_of_cinfer_ctx (S : FvSet!) :
+  --   ((x : Name) -> x ∉ S → (Γ ++ [x:A]) ⊢ {_|-> x}t >: {_|-> x}B) ->
+  --   A -β> A' ->
+  --   ((x : Name) -> x ∉ S → (Γ ++ [x:A']) ⊢ {_|-> x}t >: {_|-> x}B)
+  -- := by sorry
+
+  -- lemma preservation_step_of_cinfer_ctx_const (S : FvSet!) :
+  --   ((x : Name) -> x ∉ S → (Γ ++ [x:A]) ⊢ {_|-> x}t >: const K) ->
+  --   A -β> A' ->
+  --   ((x : Name) -> x ∉ S → (Γ ++ [x:A']) ⊢ {_|-> x}t >: const K)
+  -- := by sorry
+
+  -- lemma rule_cinfer_red : Γ ⊢ t >: A -> A -β>* B -> Γ ⊢ t >: B := by {
+  --   intro j step
+  --   cases j; case _ D j step2 =>
+  --   replace step := RedStar.trans step2 step
+  --   apply ConInfer.infer j step
+  -- }
+
+  -- lemma rule_inv_inter1_kind : ¬ (Γ ⊢ t >: inter (const K) B) := λ j => @Nat.rec
+  --   (λ s => ∀ Γ t K B,
+  --     size t ≤ s ->
+  --     ¬ Γ ⊢ t >: inter (const K) B)
+  --   sorry
+  --   (by {
+  --     intro s ih Γ t K B sh j
+  --     cases t <;> simp at *
+  --     case bound => apply ih _ (bound _) _ _ (by simp) j
+  --     case free => apply ih _ (free _) _ _ (by simp) j
+  --     case const => apply ih _ (const _) _ _ (by simp) j
+  --     case bind b u1 u2 => {
+  --       cases b <;> simp at *
+  --       case lam m => {
+  --         sorry
+  --       }
+  --       case pi m => sorry
+  --       case inter => sorry
+  --     }
+  --     case ctor => sorry
+  --   })
+  --   (size t)
+  --   Γ
+  --   t
+  --   K
+  --   B
+  --   (by simp)
+  --   j
+
+  -- lemma preservation_step_of_cinfer_const :
+  --   Γ ⊢ t >: const K ->
+  --   t -β> s ->
+  --   Γ ⊢ s >: const K
+  -- := λ j step => @ConInfer.rec
+  --   (λ Γ t A j => ∀ s K, A -β>* const K -> t -β> s -> Γ ⊢ s : A)
+  --   (λ Γ t A j => ∀ s K, A = const K -> t -β> s -> Γ ⊢ s >: A)
+  --   (λ Γ t A j => ∀ s K, A = const K -> t -β> s -> Γ ⊢ s =: A)
+  --   (λ Γ wf => True)
+  --   (by {
+  --     intro Γ wf _ s K e step
+  --     cases step
+  --   })
+  --   (by {
+  --     intro Γ x A wf xn _ s K e step
+  --     cases step
+  --   })
+  --   (by {
+  --     intro Γ A m K B S j1 j2 ih1 ih2 s K' e step; simp at *
+  --     cases step <;> simp at *
+  --     case bind1 A' step => {
+  --       cases m <;> simp at *
+  --       case free => {
+  --         have lem1 := ih1 A' Constant.typeU rfl step
+  --         have lem2 := preservation_step_of_cinfer_ctx_const S j2 step
+  --         apply @Infer.pi _ _ mf Constant.typeU _ _ lem1 lem2
+  --       }
+  --       case erased => {
+  --         have lem1 := ih1 A' K rfl step
+  --         have lem2 := preservation_step_of_cinfer_ctx_const S j2 step
+  --         apply @Infer.pi _ _ m0 K _ _ lem1 lem2
+  --       }
+  --       case type => {
+  --         have lem1 := ih1 A' K rfl step
+  --         have lem2 := preservation_step_of_cinfer_ctx_const S j2 step
+  --         apply @Infer.pi _ _ mt K _ _ lem1 lem2
+  --       }
+  --     }
+  --     case bind2 B' S' step => {
+  --       cases m <;> simp at *
+  --       case free => {
+  --         have lem2 : ∀ x, x ∉ (S ++ S') -> (Γ ++ [x:A]) ⊢ {_|-> x}B' >: typeu := by {
+  --           intro x xn; simp at xn
+  --           replace xn := demorgan xn
+  --           cases xn; case _ xn1 xn2 =>
+  --           apply ih2 x xn1 ({_|-> x}B') Constant.typeU rfl _
+  --           apply step x xn2
+  --         }
+  --         apply @Infer.pi _ _ mf Constant.typeU _ (S ++ S') j1 lem2
+  --       }
+  --       case erased => {
+  --         have lem2 : ∀ x, x ∉ (S ++ S') -> (Γ ++ [x:A]) ⊢ {_|-> x}B' >: typeu := by {
+  --           intro x xn; simp at xn
+  --           replace xn := demorgan xn
+  --           cases xn; case _ xn1 xn2 =>
+  --           apply ih2 x xn1 ({_|-> x}B') Constant.typeU rfl _
+  --           apply step x xn2
+  --         }
+  --         apply @Infer.pi _ _ m0 K _ (S ++ S') j1 lem2
+  --       }
+  --       case type => {
+  --         have lem2 : ∀ x, x ∉ (S ++ S') -> (Γ ++ [x:A]) ⊢ {_|-> x}B' >: kindu := by {
+  --           intro x xn; simp at xn
+  --           replace xn := demorgan xn
+  --           cases xn; case _ xn1 xn2 =>
+  --           apply ih2 x xn1 ({_|-> x}B') Constant.kindU rfl _
+  --           apply step x xn2
+  --         }
+  --         apply @Infer.pi _ _ mt K _ (S ++ S') j1 lem2
+  --       }
+  --     }
+  --   })
+  --   sorry
+  --   sorry
+  --   sorry
+  --   (sorry)
+  --   (by {
+  --     intro Γ t A B j ih s K e step
+  --     sorry
+  --   })
+  --   sorry
+  --   (by {
+  --     intro Γ A a b j1 j2 j3 ih1 ih2 ih3 s K e step
+  --     cases step <;> simp at *
+  --     case ctor1 => sorry
+  --     case ctor2 a' step => {
+  --       sorry
+  --     }
+  --     case ctor3 => sorry
+  --   })
+  --   sorry
+  --   sorry
+  --   sorry
+  --   sorry
+  --   sorry
+  --   (by {
+  --     intro Γ t A B j step ih s K e step'
+  --     subst e
+  --     have lem := ih s K step step'
+  --     apply ConInfer.infer lem step
+  --   })
+  --   (by {
+  --     intro Γ t A B K' j1 j2 conv ih1 ih2 s K e step
+  --     subst e;
+  --     cases conv; case _ A' K'' S s1 er s2 =>
+  --     cases s2
+  --     case refl => {
+  --       clear ih2
+  --       sorry
+  --     }
+  --     case step _ step _ => cases step
+  --   })
+  --   (by simp)
+  --   (by simp)
+  --   Γ
+  --   t
+  --   (const K)
+  --   j
+  --   s
+  --   K
+  --   rfl
+  --   step
+
+
+  -- lemma preservation_step_of_cinfer_pi_domain :
+  --   Γ ⊢ t >: Mode.pi_domain m K ->
+  --   t -β> s ->
+  --   Γ ⊢ s >: Mode.pi_domain m K
+  -- := λ j step => @Nat.rec
+  --   (λ si => ∀ Γ t m K s,
+  --     size t ≤ si ->
+  --     Γ ⊢ t >: Mode.pi_domain m K ->
+  --     t -β> s ->
+  --     Γ ⊢ s >: Mode.pi_domain m K)
+  --   sorry
+  --   (by {
+  --     intro si ih Γ t m K s sh j step
+  --     cases t <;> simp at *
+  --     case bound => cases step
+  --     case free => cases step
+  --     case const => cases step
+  --     case bind b u1 u2 => {
+  --       have s1 : size u1 ≤ si := by linarith
+  --       have s2 : size u2 ≤ si := by linarith
+  --       cases b <;> simp at *
+  --       case lam m' => {
+  --         cases j; case _ D j step2 =>
+  --         cases j; case _ K2 B2 S2 j1 j2 j3 =>
+  --         exfalso; apply red_inv_pi_not_pi_domain step2
+  --       }
+  --       case pi m' => {
+  --         cases j; case _ D j step2 =>
+  --         cases j; case _ K2 S2 j1 j2 =>
+  --         have e := red_force_mode_pi_codomain step2; rw [e]
+  --         cases step <;> simp
+  --         case bind1 u1' step => {
+  --           cases m' <;> simp at *
+  --           case free => {
+  --             have lem := @ih Γ u1 mf Constant.typeU u1' s1 j1 step; simp at lem
+  --             apply ConInfer.infer _ _; exact typeu
+  --             apply @Infer.pi _ _ mf Constant.typeU _ S2 lem
+  --             simp; apply preservation_step_of_cinfer_ctx_const S2 j2 step
+  --             apply RedStar.refl
+  --           }
+  --           case erased => sorry
+  --           case type => sorry
+  --         }
+  --         case bind2 => sorry
+  --       }
+  --       case inter => {
+  --         cases j; case _ D j step2 =>
+  --         cases j; case _ S2 j1 j2 =>
+  --         have e := red_force_typeu step2; rw [e]
+  --         cases step <;> simp
+  --         case bind1 u1' step => {
+  --           have lem := @ih Γ u1 mf K u1' s1 j1 step; simp at lem
+  --           sorry
+  --         }
+  --         case bind2 => sorry
+  --       }
+  --     }
+  --     case ctor c u1 u2 u3 => {
+  --       have s1 : size u1 ≤ si := by linarith
+  --       have s2 : size u2 ≤ si := by linarith
+  --       have s3 : size u3 ≤ si := by linarith
+  --       cases c <;> simp at *
+  --       case app m => sorry
+  --       case pair => {
+  --         cases j; case _ D j step2 =>
+  --         cases j; case _ A B j1 j2 j3 j4 =>
+  --         exfalso; apply red_inv_inter_not_pi_domain step2
+  --       }
+  --       case fst => {
+  --         cases j; case _ D j step2 =>
+  --         cases j; case _ B j =>
+  --         have step2 : inter D B -β>* inter (Mode.pi_domain m K) B := by {
+  --           apply red_inter' step2 (λ _ _ => RedStar.refl); exact []
+  --         }
+  --         replace j := rule_cinfer_red j step2
+  --         cases m <;> simp at *
+  --         case free => exfalso; apply rule_inv_inter1_kind j
+  --         case erased => exfalso; apply rule_inv_inter1_kind j
+  --         case type => exfalso; apply rule_inv_inter1_kind j
+  --       }
+  --       case snd => sorry
+  --       case eq => sorry
+  --       case refl => sorry
+  --       case eqind => sorry
+  --       case j0 => sorry
+  --       case jω => sorry
+  --       case promote => sorry
+  --       case delta => sorry
+  --       case phi => sorry
+  --     }
+  --   })
+  --   (size t)
+  --   Γ
+  --   t
+  --   m
+  --   K
+  --   s
+  --   (by simp)
+  --   j
+  --   step
+
+
+  -- lemma preservation_of_infer_step4 : Γ ⊢ t : A -> t -β> s -> Γ ⊢ s : A := by {
+  --   intro j step
+  --   induction step generalizing Γ A
+  --   case beta m u1 u2 u3 => {
+  --     cases j; case _ A B S j1 j2 =>
+  --     sorry
+  --   }
+  --   case fst u1 u2 u3 => {
+  --     cases j; case _ B j =>
+  --     cases j; case _ T j step =>
+  --     sorry
+  --   }
+  --   case snd => sorry
+  --   case eqind => sorry
+  --   case promote => sorry
+  --   case phi => sorry
+  --   case bind1 => sorry
+  --   case bind2 => sorry
+  --   case ctor1 => sorry
+  --   case ctor2 => sorry
+  --   case ctor3 => sorry
+  -- }
+
+  -- lemma preservation_of_infer_step : Γ ⊢ t : A -> t -β> s -> ∃ B, Γ ⊢ s : B := by {
+  --   intro tproof step
+  --   induction step generalizing Γ A
+  --   case beta m u1 u2 u3 => {
+  --     cases tproof; case _ A B S j1 j2 =>
+  --     apply preservation_of_infer_step_subst j1 j2
+  --   }
+  --   case fst u1 u2 u3 => {
+  --     cases tproof; case _ B j =>
+  --     cases j; case _ P j step =>
+  --     cases j; case _ A2 B2 j1 j2 j3 j4 =>
+  --     cases j1; case _ A3 j5 j6 =>
+  --     sorry
+  --   }
+  --   case snd u1 u2 u3 => {
+  --     cases tproof; case _ A1 B1 j =>
+  --     cases j; case _ P j1 s1 =>
+  --     cases j1; case _ A2 B2 j1 j2 j3 j4 =>
+  --     cases j3; case _ A3 j5 c1 =>
+  --     sorry
+  --   }
+  --   case eqind u1 u2 u3 u4 u5 u6 => {
+  --     cases tproof
+  --     case eqind j1 j2 j3 j4 j5 j6 => {
+  --       cases j5; case _ D j5 c1 =>
+  --       cases j5; case _ A j =>
+  --       sorry
+  --     }
+  --   }
+  --   case promote u => {
+  --     cases tproof; case _ T a b A B j1 j2 =>
+  --     cases j2; case _ A2 j2 s1 =>
+  --     cases j2; case _ A3 j2 =>
+  --     cases j2; case _ B2 j2 =>
+  --     cases j2; case _ T j s2 =>
+  --     exists eq T u u
+  --     apply Infer.refl; simp [*]
+  --   }
+  --   case phi => sorry
+  --   case bind1 u1 u2 k u3 s1 ih => {
+  --     cases k <;> simp at *
+  --     case lam m => {
+  --       cases tproof; case _ K B S j1 j2 j3 =>
+  --       cases j1; case _ T j1 step2 =>
+  --       have lem := ih j1
+  --       cases lem; case _ D jlem =>
+  --       have cj1 : Γ ⊢ u1 >: Mode.pi_domain m K := ConInfer.infer j1 step2
+  --       have lem1 := preservation_step_of_cinfer_pi_domain cj1 s1
+  --       have lem2 := @preservation_step_of_infer_ctx Γ u1 u3 B u2 S j3 s1
+  --       cases lem2; case _ B' lem2 =>
+  --       exists (pi m u2 B')
+  --       apply Infer.lam lem1 lem2 j2
+  --     }
+  --     case pi m => sorry
+  --     case inter => sorry
+  --   }
+  --   case bind2 u1 u2 k u3 S1 s1 ih => {
+  --     cases k <;> simp at *
+  --     case lam m => {
+  --       cases tproof; case _ K B S2 j1 j2 j3 =>
+  --       have xfresh := @Name.fresh_is_fresh (S1 ++ S2)
+  --       generalize xdef : Name.fresh (S1 ++ S2) = x at *
+  --       simp at *
+  --       replace xfresh := demorgan xfresh
+  --       cases xfresh; case _ xn1 xn2 =>
+  --       have lem1 := ih x xn1 (j3 x xn2)
+  --       cases lem1; case _ D lem1 =>
+  --       have lem2 := to_open D x
+  --       cases lem2; case _ D' lem2 =>
+  --       subst lem2
+  --       exists pi m u3 D'
+  --       apply Infer.lam j1 _ _
+  --       exact S2; intro y yn
+  --       sorry
+
+
+  --       sorry
+  --     }
+  --     case pi m => sorry
+  --     case inter => sorry
+  --   }
+  --   case ctor1 => sorry
+  --   case ctor2 => sorry
+  --   case ctor3 => sorry
+  -- }
+
+  -- lemma preservation_of_infer_step3 : Γ ⊢ t : A -> t -β> s -> ∃ B, Γ ⊢ s : B
+  --   := λ j step => @Infer.rec
+  --     (λ Γ t A j' => ∀ s, t -β> s -> ∃ B, Γ ⊢ s : B)
+  --     (λ Γ t A j' => ∀ s, t -β> s -> ∃ B, Γ ⊢ s >: B)
+  --     (λ Γ t A j' => ∀ s, t -β> s -> ∃ B, Γ ⊢ s =: B)
+  --     (λ Γ wf => True)
+  --   sorry
+  --   sorry
+  --   sorry
+  --   (by {
+  --     intro Γ A m K t B S j1 j2 j3 ih1 ih2 s step; simp at *
+  --     cases step <;> simp
+  --     case bind1 A' step => {
+  --       sorry
+  --     }
+  --     case bind2 => sorry
+  --   })
+  --   sorry
+  --   sorry
+  --   sorry
+  --   sorry
+  --   sorry
+  --   sorry
+  --   sorry
+  --   sorry
+  --   sorry
+  --   sorry
+  --   sorry
+  --   (by {
+  --     intro Γ t A B j step ih s step2
+  --     have lem := ih s step2
+  --     cases lem; case _ D j2 =>
+  --     sorry
+  --   })
+  --   (by {
+  --     intro Γ t A B j c ih s step
+  --     sorry
+  --   })
+  --   sorry
+  --   sorry
+  --   Γ
+  --   t
+  --   A
+  --   j
+  --   s
+  --   step
+
+  -- theorem preservation_of_infer : Γ ⊢ t : A -> t -β>* s -> ∃ B, Γ ⊢ s : B := sorry
 
 end Cedille
