Cedille/Lemma/Conv.lean
@@ -1,7 +1,8 @@
 
-import Cedille.Def 
+import Cedille.Def
 import Cedille.Lemma.Erasure
 import Cedille.Lemma.Red
+import Cedille.Lemma.RedErasure
 import Cedille.Lemma.Confluence
 
 namespace Cedille.BetaConv
@@ -102,9 +103,55 @@ namespace Cedille.Conv
     apply BetaConv.symm (e x)
   }
 
-  lemma by_beta (S : FvSet!) : (∀ x, erase x a =β= erase x b) -> a === b := by {
+  lemma by_beta : (∀ x, erase x a =β= erase x b) -> a === b := by {
     intro h
     apply Conv.conv RedStar.refl RedStar.refl h
+  }
+
+  lemma red_f :
+    Sane a ->
+    a === b ->
+    a -β>* a' ->
+    a' === b
+  := by {
+    intro h cv step
+    cases cv; case _ u v r1 e r2 =>
+    have lem1 := confluence step r1
+    casesm* ∃ _, _, _ ∧ _; case _ z r3 r4 =>
+    have lem2 := preservation_of_sanity h r1
+    replace e := erase_red_f lem2 e r4
+    constructor; exact r3; exact r2; exact e
+  }
+
+  lemma trans :
+    Sane B ->
+    A === B ->
+    B === C ->
+    A === C
+  := by {
+    intro h c1 c2
+    cases c1; case _ u1 u2 r1 e1 r2 =>
+    cases c2; case _ v1 v2 r3 e2 r4 =>
+    have lem := confluence r2 r3
+    casesm* ∃ _, _, _ ∧ _; case _ B' rr1 rr2 =>
+    constructor; exact r1; exact r4
+    intro x
+    have h2 : Sane u2 := preservation_of_sanity h r2
+    have h3 : Sane v1 := preservation_of_sanity h r3
+    replace e1 := erase_red_f h2 (λ x => BetaConv.symm (e1 x)) rr1
+    replace e2 := erase_red_f h3 e2 rr2
+    have lem := BetaConv.trans (BetaConv.symm (e1 x)) (e2 x)
+    exact lem
+  }
+
+  lemma to_beta (S : FvSet!) : Sane a -> Sane b -> a === b -> (∀ x, erase x a =β= erase x b)
+  := by {
+    intro h1 h2 cv
+    cases cv; case _ a' b' r1 e r2 =>
+    intro x;
+    replace e := erase_red_b h1 e r1
+    replace e := erase_red_b h2 (λ x => BetaConv.symm (e x)) r2
+    apply BetaConv.symm (e x)
   }
 
 end Cedille.Conv
