Cedille/Lemma/RedErasure.lean
@@ -6,17 +6,226 @@ import Cedille.Lemma.Refold
 import Cedille.Lemma.Erasure
 import Cedille.Lemma.Inversion
 import Cedille.Lemma.Red
-import Cedille.Lemma.Confluence
-import Cedille.Lemma.Conv
-import Cedille.Lemma.Preservation
 
 namespace Cedille
 
-  lemma erase_free_red :
-    ((x : Name) -> x ∉ fv t -> x ∉ (fv ∘ erase x) ({_|-> x}t)) ->
-    (∃ x, {_|-> x}t -β>* {_|-> x}t') ->
-    (x : Name) -> x ∉ fv t' -> x ∉ (fv ∘ erase x) ({_|-> x}t')
-  := sorry
+  lemma erase_red_f_step :
+    Sane a ->
+    (∀ x, erase x a =β= erase x b) ->
+    a -β> a' ->
+    (∀ x, erase x a' =β= erase x b)
+  := by {
+    intro j e step
+    induction j generalizing a' b
+    case ax => cases step
+    case var => cases step
+    case pi => sorry
+    case lam A t m S Ah th tfv Aih tih => {
+      cases step
+      case bind1 A' step => {
+        simp at *
+        sorry
+      }
+      case bind2 t' S' step => {
+        simp at *
+        sorry
+      }
+    }
+    case app f a m fh ah fih aih => {
+      cases step
+      case beta c t1 t2 => {
+        sorry
+      }
+      case ctor1 f' step => {
+        simp at *
+        sorry
+      }
+      case ctor2 a' step => {
+        simp at *
+        sorry
+      }
+      case ctor3 _ step => cases step
+    }
+    case inter => sorry
+    case pair T t s Th th sh e2 Tih tih sih => {
+      cases step
+      case ctor1 t' step => {
+        simp at *
+        apply tih e step
+      }
+      case ctor2 s' step => {
+        simp at *
+        apply e
+      }
+      case ctor3 T' step => {
+        simp at *; apply e
+      }
+    }
+    case fst t h ih => {
+      cases step
+      case fst u v => {
+        intro x; replace e := e x
+        rw [erase_fst, erase_pair] at e
+        exact e
+      }
+      case phi u v => {
+        intro x; replace e := e x
+        rw [erase_fst, erase_phi] at e
+        exact e
+      }
+      case ctor1 t' step => {
+        simp at *; apply ih e step
+      }
+      case ctor2 _ step => cases step
+      case ctor3 _ step => cases step
+    }
+    case snd t h ih => {
+      cases step
+      case snd u v => {
+        simp at *
+        cases h; case _ h1 h2 e2 h3 =>
+        -- Holds by transitivity of =β=
+        sorry
+      }
+      case ctor1 t' step => {
+        simp at *
+        apply ih e step
+      }
+      case ctor2 _ step => cases step
+      case ctor3 _ step => cases step
+    }
+    case eq T x y Th xh yh Tih xih yih => {
+      cases step
+      case ctor1 T' step => {
+        simp at *
+        sorry
+      }
+      case ctor2 => sorry
+      case ctor3 => sorry
+    }
+    case refl t h ih => {
+      cases step
+      case ctor1 t' step => {
+        simp at *; apply e
+      }
+      case ctor2 _ step => cases step
+      case ctor3 _ step => cases step
+    }
+    case eqind A P x y r w Ah Ph xh yh rh wh Aih Pih xih yih rih wih => {
+      cases step
+      case eqind t => {
+        simp at *
+        sorry -- Easy, by β
+      }
+      case ctor1 t' step => simp at *; apply e
+      case ctor2 => simp at *; apply e
+      case ctor3 t' step => {
+        simp at *
+        cases step
+        case ctor1 r' step => {
+          sorry
+        }
+        case ctor2 w' step => sorry
+        case ctor3 _ step  => cases step
+      }
+    }
+    case promote t h ih => {
+      cases step
+      case promote t => {
+        intro x; replace e := e x
+        rw [erase_promote, erase_refl] at e
+        simp [*]
+      }
+      case ctor1 t' step => {
+        simp at *
+        apply ih e step
+      }
+      case ctor2 _ step => cases step
+      case ctor3 _ step => cases step
+    }
+    case phi c f t ch fh th cih fih tih => {
+      cases step
+      case ctor1 c' step => {
+        simp at *
+        apply cih e step
+      }
+      case ctor2 f' step => {
+        simp at *; apply e
+      }
+      case ctor3 t' step => simp at *; apply e
+    }
+    case delta t h ih => {
+      cases step
+      case ctor1 t' step => {
+        simp at *
+        apply ih e step
+      }
+      case ctor2 _ step => cases step
+      case ctor3 _ step => cases step
+    }
+  }
+
+  lemma erase_red_f :
+    Sane a ->
+    (∀ x, erase x a =β= erase x b) ->
+    a -β>* a' ->
+    (∀ x, erase x a' =β= erase x b)
+  := by {
+    intro j e step
+    induction step
+    case refl => simp [*]
+    case step t1 t2 _t3 r1 _r2 ih => {
+      have lem1 := preservation_of_sanity_step j r1
+      have lem2 := erase_red_f_step j e r1
+      apply ih lem1 lem2
+    }
+  }
+
+  lemma erase_red_b_step :
+    Sane a ->
+    (∀ x, erase x a' =β= erase x b) ->
+    a -β> a' ->
+    (∀ x, erase x a =β= erase x b)
+  := by {
+    intro h e step
+    induction h generalizing b
+    case ax => sorry
+    case var => sorry
+    case pi => sorry
+    case lam => sorry
+    case app => sorry
+    case inter => sorry
+    case pair => sorry
+    case fst => sorry
+    case snd => sorry
+    case eq => sorry
+    case refl => sorry
+    case eqind => sorry
+    case promote => sorry
+    case phi => sorry
+    case delta => sorry
+  }
+
+  lemma erase_red_b :
+    Sane a ->
+    (∀ x, erase x a' =β= erase x b) ->
+    a -β>* a' ->
+    (∀ x, erase x a =β= erase x b)
+  := by {
+    intro h e step
+    induction step
+    case refl t => simp [*]
+    case step u v w r1 _r2 ih => {
+      have h2 := preservation_of_sanity_step h r1
+      have lem := ih h2 e
+      apply erase_red_b_step h lem r1
+    }
+  }
+  -- lemma erase_free_red :
+  --   ((x : Name) -> x ∉ fv t -> x ∉ (fv ∘ erase x) ({_|-> x}t)) ->
+  --   (∃ x, {_|-> x}t -β>* {_|-> x}t') ->
+  --   (x : Name) -> x ∉ fv t' -> x ∉ (fv ∘ erase x) ({_|-> x}t')
+  -- := sorry
 
   -- lemma red_erasure_step_lam_mf :
   --   erase t1 = lam mf kindu (erase t2) ->
@@ -82,7 +291,7 @@ namespace Cedille
   --   t1 -β> z1 ->
   --   ∃ z2, t2 -β>* z2 ∧ erase z1 = erase z2
   -- := λ j1 j2 h step => @Nat.rec
-  --   (λ n => 
+  --   (λ n =>
   --     ∀ Γ1 t1 A1 Γ2 t2 A2 z1,
   --     size t2 ≤ n ->
   --     Γ1 ⊢ t1 : A1 ->
@@ -198,7 +407,7 @@ namespace Cedille
   --   t1 -β> z1 ->
   --   ∃ z2, t2 -β>* z2 ∧ erase z1 = erase z2
   -- := λ h step => @Nat.rec
-  --   (λ n => 
+  --   (λ n =>
   --     ∀ m (t1 t2 z1 : Term m),
   --     size t1 ≤ n ->
   --     erase t1 = erase t2 ->
@@ -226,7 +435,7 @@ namespace Cedille
   --             generalize xdef : Name.fresh S = x at *
   --             replace step := step x fresh
   --             have lem := ih m ({_|-> x}u2) (t2) ({_|-> x}v2) sorry sorry step
-              
+
   --           }
   --         }
   --         case type => {
@@ -256,144 +465,144 @@ namespace Cedille
   --   h
   --   step
 
-  lemma typed_fv_erase :
-    Γ ⊢ a : A ->
-    x ∉ fv (erase x a)
-  := sorry
+  -- lemma typed_fv_erase :
+  --   Γ ⊢ a : A ->
+  --   x ∉ fv (erase x a)
+  -- := sorry
 
-  lemma typed_fv_erase_bind (S : FvSet!) :
-    (∀ x, x ∉ S -> (Γ ++ [x:C]) ⊢ {_|-> x}a >: A) ->
-    x ∉ fv (erase x a)
-  := sorry
+  -- lemma typed_fv_erase_bind (S : FvSet!) :
+  --   (∀ x, x ∉ S -> (Γ ++ [x:C]) ⊢ {_|-> x}a >: A) ->
+  --   x ∉ fv (erase x a)
+  -- := sorry
 
-  lemma red_erase_step :
-    Γ ⊢ a : A ->
-    a -β> b ->
-    (∀ x, erase x a =β= erase x b)
-  := λ j step => @Infer.rec
-    (λ Γ a A j => ∀ b,
-      a -β> b ->
-      (∀ x, erase x a =β= erase x b))
-    (λ Γ a A j => ∀ b,
-      a -β> b ->
-      (∀ x, erase x a =β= erase x b))
-    (λ Γ a A j => ∀ b,
-      a -β> b ->
-      (∀ x, erase x a =β= erase x b))
-    (λ Γ wf => True)
-    (by {
-      intro Γ wf _ b step
-      cases step
-    })
-    (by {
-      intro Γ y C wf yn _ b step
-      cases step
-    })
-    sorry
-    sorry
-    sorry
-    (by {
-      simp at *
-      intro Γ C B S j1 j2 ih1 ih2 b step
-      cases step
-      case bind1 C' step => {
-        simp at *
-        replace ih1 := ih1 C' step
-        intro x
-        apply BetaConv.bind x (ih1 x) _ BetaConv.refl
-        intro h; simp at h
-        apply typed_fv_erase_bind S j2 h
-      }
-      case bind2 B' S' step => {
-        sorry
-      }
-    })
-    sorry
-    (by {
-      simp
-      intro Γ t A B j ih b r x
-      cases r <;> simp
-      case fst => apply BetaConv.refl
-      case phi t2 t3 => apply BetaConv.refl
-      case ctor1 => sorry
-      case ctor2 => sorry
-      case ctor3 => sorry
-    })
-    (by {
-      simp
-      intro Γ t C B j ih b r
-      cases r
-      case snd t1 t3 => {
-        cases j; case _ _ j _ =>
-        cases j; case _ S2 _ e _ _ _ =>
-        simp [*]
-      }
-      case ctor1 => sorry
-      case ctor2 => sorry
-      case ctor3 => sorry
-    })
-    sorry
-    sorry
-    sorry
-    sorry
-    (by {
-      simp at *
-      intro Γ f A B a e j1 j2 j3 j4 ih1 ih2 ih3 b r x
-      cases r <;> simp
-      case ctor1 a' r => apply ih2 a' r x
-      case ctor2 f' r => apply BetaConv.refl
-      case ctor3 => apply BetaConv.refl
-    })
-    (by {
-      simp
-      intro Γ e j ih b r x
-      cases r <;> simp
-      case ctor1 e' r => apply ih e' r x
-      case ctor2 _ r => cases r
-      case ctor3 _ r => cases r
-    })
-    sorry
-    sorry
-    sorry
-    sorry
-    Γ
-    a
-    A
-    j
-    b
-    step
+  -- lemma red_erase_step :
+  --   Γ ⊢ a : A ->
+  --   a -β> b ->
+  --   (∀ x, erase x a =β= erase x b)
+  -- := λ j step => @Infer.rec
+  --   (λ Γ a A j => ∀ b,
+  --     a -β> b ->
+  --     (∀ x, erase x a =β= erase x b))
+  --   (λ Γ a A j => ∀ b,
+  --     a -β> b ->
+  --     (∀ x, erase x a =β= erase x b))
+  --   (λ Γ a A j => ∀ b,
+  --     a -β> b ->
+  --     (∀ x, erase x a =β= erase x b))
+  --   (λ Γ wf => True)
+  --   (by {
+  --     intro Γ wf _ b step
+  --     cases step
+  --   })
+  --   (by {
+  --     intro Γ y C wf yn _ b step
+  --     cases step
+  --   })
+  --   sorry
+  --   sorry
+  --   sorry
+  --   (by {
+  --     simp at *
+  --     intro Γ C B S j1 j2 ih1 ih2 b step
+  --     cases step
+  --     case bind1 C' step => {
+  --       simp at *
+  --       replace ih1 := ih1 C' step
+  --       intro x
+  --       apply BetaConv.bind x (ih1 x) _ BetaConv.refl
+  --       intro h; simp at h
+  --       apply typed_fv_erase_bind S j2 h
+  --     }
+  --     case bind2 B' S' step => {
+  --       sorry
+  --     }
+  --   })
+  --   sorry
+  --   (by {
+  --     simp
+  --     intro Γ t A B j ih b r x
+  --     cases r <;> simp
+  --     case fst => apply BetaConv.refl
+  --     case phi t2 t3 => apply BetaConv.refl
+  --     case ctor1 => sorry
+  --     case ctor2 => sorry
+  --     case ctor3 => sorry
+  --   })
+  --   (by {
+  --     simp
+  --     intro Γ t C B j ih b r
+  --     cases r
+  --     case snd t1 t3 => {
+  --       cases j; case _ _ j _ =>
+  --       cases j; case _ S2 _ e _ _ _ =>
+  --       simp [*]
+  --     }
+  --     case ctor1 => sorry
+  --     case ctor2 => sorry
+  --     case ctor3 => sorry
+  --   })
+  --   sorry
+  --   sorry
+  --   sorry
+  --   sorry
+  --   (by {
+  --     simp at *
+  --     intro Γ f A B a e j1 j2 j3 j4 ih1 ih2 ih3 b r x
+  --     cases r <;> simp
+  --     case ctor1 a' r => apply ih2 a' r x
+  --     case ctor2 f' r => apply BetaConv.refl
+  --     case ctor3 => apply BetaConv.refl
+  --   })
+  --   (by {
+  --     simp
+  --     intro Γ e j ih b r x
+  --     cases r <;> simp
+  --     case ctor1 e' r => apply ih e' r x
+  --     case ctor2 _ r => cases r
+  --     case ctor3 _ r => cases r
+  --   })
+  --   sorry
+  --   sorry
+  --   sorry
+  --   sorry
+  --   Γ
+  --   a
+  --   A
+  --   j
+  --   b
+  --   step
 
-  lemma red_erase :
-    Γ ⊢ a : A ->
-    a -β>* b ->
-    (∀ x, erase x a =β= erase x b)
-  := by {
-    intro j step x
-    induction step generalizing Γ A
-    case refl => apply BetaConv.refl
-    case step t1 t2 t3 step _ ih => {
-      have jt2 := preservation_of_infer_step j step
-      cases jt2; case _ U j2 =>
-      replace ih := ih j2
-      have lem := red_erase_step j step
-      apply BetaConv.trans (lem x) ih
-    }
-  }
+  -- lemma red_erase :
+  --   Γ ⊢ a : A ->
+  --   a -β>* b ->
+  --   (∀ x, erase x a =β= erase x b)
+  -- := by {
+  --   intro j step x
+  --   induction step generalizing Γ A
+  --   case refl => apply BetaConv.refl
+  --   case step t1 t2 t3 step _ ih => {
+  --     have jt2 := preservation_of_infer_step j step
+  --     cases jt2; case _ U j2 =>
+  --     replace ih := ih j2
+  --     have lem := red_erase_step j step
+  --     apply BetaConv.trans (lem x) ih
+  --   }
+  -- }
 
-  theorem conv_by_erase :
-    Γ1 ⊢ a : A ->
-    Γ2 ⊢ b : B -> 
-    a === b ->
-    (∀ x, erase x a =β= erase x b)
-  := by {
-    intro ja jb cv x
-    cases cv; case _ u v r1 e r2 =>
-    have lem1 := red_erase ja r1
-    have lem2 := red_erase jb r2
-    have e2 := BetaConv.trans (lem1 x) (e x)
-    apply BetaConv.trans e2
-    apply BetaConv.symm (lem2 x)
-  }
+  -- theorem conv_by_erase :
+  --   Γ1 ⊢ a : A ->
+  --   Γ2 ⊢ b : B ->
+  --   a === b ->
+  --   (∀ x, erase x a =β= erase x b)
+  -- := by {
+  --   intro ja jb cv x
+  --   cases cv; case _ u v r1 e r2 =>
+  --   have lem1 := red_erase ja r1
+  --   have lem2 := red_erase jb r2
+  --   have e2 := BetaConv.trans (lem1 x) (e x)
+  --   apply BetaConv.trans e2
+  --   apply BetaConv.symm (lem2 x)
+  -- }
 
   -- lemma red_erasure (S : FvSet!) :
   --   Γ1 ⊢ t1 : A1 ->
