Cedille/Lemma/Substitution.lean
@@ -1,0 +1,20 @@
+import Cedille.Def
+import Cedille.Lemma.Basic
+import Cedille.Lemma.Refold
+import Cedille.Lemma.Erasure
+import Cedille.Lemma.Inversion
+import Cedille.Lemma.Syntax
+
+namespace Cedille
+
+  lemma subst_hsubst_commute {t1 t2 : Term n} {t3 : Term (n + 1)} :
+    [x := t1][_:= t2]t3 = [_:= [x := t1]t2][x := t1ʷ]t3
+  := by sorry
+
+  lemma sanity_subst {S : FvSet!} :
+    Sane a ->
+    (∀ x, x ∉ S -> Sane ({_|-> x}f)) ->
+    Sane ([_:= a]f)
+  := by sorry
+
+end Cedille
