Common/Util.lean
@@ -11,6 +11,25 @@ lemma demorgan : ¬ (A ∨ B) -> ¬ A ∧ ¬ B := by {
   intro h2; apply h (Or.inr h2)
 }
 
+lemma demorgan3 : ¬ (A ∨ B ∨ C) -> ¬ A ∧ ¬ B ∧ ¬ C := by {
+  intro h
+  have lem := demorgan h
+  cases lem; case _ h1 h2 =>
+  have lem2 := demorgan h2
+  cases lem2; case _ h3 h4 =>
+  apply And.intro h1 _
+  apply And.intro h3 h4
+}
+
+lemma demorgan4 : ¬ (A ∨ B ∨ C ∨ D) -> ¬ A ∧ ¬ B ∧ ¬ C ∧ ¬ D := by {
+  intro h
+  have lem := demorgan3 h
+  casesm* _ ∧ _; case _ h1 h2 h3 =>
+  have lem2 := demorgan h3
+  cases lem2; case _ h4 h5 =>
+  apply And.intro h1 (And.intro h2 (And.intro h4 h5))
+}
+
 def ne_sym : x ≠ y -> y ≠ x := by intro h1 h2; subst h2; contradiction
 
 def append_eq {a c : List α} {b d : α} : a ++ [b] = c ++ [d] -> a = c ∧ b = d := by {
@@ -51,7 +70,7 @@ def fin_cast {i : Nat} : (h : i < i + 1) -> Fin.mk i h = ↑i := by {
     have lem2 := (@Nat.mod_eq_iff_lt x _ lem1).2 (by linarith)
     have lem3 : (Nat.succ x + 1) ≠ 0 := by linarith
     have lem4 := (@Nat.mod_eq_iff_lt (x + 1) _ lem3).2 (by linarith)
-    rw [lem2, lem4]  
+    rw [lem2, lem4]
   }
 }
 
